cleanup

thy/Iptables_Semantics/Semantics_Ternary/Primitive_Normalization.thy
@@ -674,13 +674,14 @@ lemma not_has_disc_normalize_match:
   using i_m_giving_this_a_funny_name_so_i_can_thank_my_future_me_when_sledgehammer_will_find_this_one_day by blast
 
 lemma normalize_match_preserves_normalized_n_primitive:
-  "normalized_n_primitive (disc, sel) f rst \<Longrightarrow>
-        \<forall> r \<in> set (normalize_match rst). normalized_n_primitive (disc, sel) f r"
+  "normalized_n_primitive disc_sel f rst \<Longrightarrow>
+        \<forall> m \<in> set (normalize_match rst). normalized_n_primitive disc_sel f m"
+apply(cases disc_sel, simp)
 apply(induction rst rule: normalize_match.induct)
       apply(simp; fail)
      apply(simp; fail)
     apply(simp; fail)
-   using normalized_n_primitive.simps(5) apply blast (*simp loops*)
+   using normalized_n_primitive.simps(5) apply metis (*simp loops*)
   by simp+
 
 
@@ -869,5 +870,97 @@ subsection\<open>Optimizing a match expression\<close>
                  normalized_n_primitive.simps(4) by blast 
         with goal1 show ?thesis by simp
    qed
+
+
+
+subsection\<open>Processing a list of normalization functions\<close>
+
+fun compress_normalize_primitive_monad :: "('a match_expr \<Rightarrow> 'a match_expr option) list \<Rightarrow> 'a match_expr \<Rightarrow> 'a match_expr option" where
+  "compress_normalize_primitive_monad [] m = Some m" |
+  "compress_normalize_primitive_monad (f#fs) m = (case f m of None \<Rightarrow> None
+                                                           |  Some m' \<Rightarrow> compress_normalize_primitive_monad fs m')"
+
+lemma compress_normalize_primitive_monad: 
+      assumes "\<And>m m' f. f \<in> set fs \<Longrightarrow> normalized_nnf_match m \<Longrightarrow> f m = Some m' \<Longrightarrow> matches \<gamma> m' a p \<longleftrightarrow> matches \<gamma> m a p"
+          and "\<And>m m' f. f \<in> set fs \<Longrightarrow> normalized_nnf_match m \<Longrightarrow> f m = Some m' \<Longrightarrow> normalized_nnf_match m'"
+          and "normalized_nnf_match m"
+          and "(compress_normalize_primitive_monad fs m) = Some m'"
+      shows "matches \<gamma> m' a p \<longleftrightarrow> matches \<gamma> m a p" (is ?goal1)
+        and "normalized_nnf_match m'"              (is ?goal2)
+  proof -
+    (*everything in one big induction*)
+    have goals: "?goal1 \<and> ?goal2"
+    using assms proof(induction fs arbitrary: m)
+    case Nil thus ?case by simp
+    next
+    case (Cons f fs)
+      from Cons.prems(1) have IH_prem1:
+        "(\<And>f m m'. f \<in> set fs \<Longrightarrow> normalized_nnf_match m \<Longrightarrow> f m = Some m' \<Longrightarrow> matches \<gamma> m' a p = matches \<gamma> m a p)" by auto
+      from Cons.prems(2) have IH_prem2:
+        "(\<And>f m m'. f \<in> set fs \<Longrightarrow> normalized_nnf_match m \<Longrightarrow> f m = Some m' \<Longrightarrow> normalized_nnf_match m')" by auto
+      from Cons.IH IH_prem1 IH_prem2 have
+        IH: "\<And>m. normalized_nnf_match m \<Longrightarrow> compress_normalize_primitive_monad fs m = Some m' \<Longrightarrow>
+                  (matches \<gamma> m' a p \<longleftrightarrow> matches \<gamma> m a p) \<and> ?goal2" by fast
+      show ?case
+        proof(cases "f m")
+          case None thus ?thesis using Cons.prems by auto
+        next
+          case(Some m'')
+            from Some Cons.prems(1)[of f] Cons.prems(3) have 1: "matches \<gamma> m'' a p = matches \<gamma> m a p" by simp
+            from Some Cons.prems(2)[of f] Cons.prems(3) have 2: "normalized_nnf_match m''" by simp
+            from Some have "compress_normalize_primitive_monad (f # fs) m = compress_normalize_primitive_monad fs m''" by simp
+            thus ?thesis using Cons.prems(4) IH 1 2 by auto 
+        qed
+    qed
+    from goals show ?goal1 by simp
+    from goals show ?goal2 by simp
+  qed
+
+(*proof is a bit sledgehammered*)
+lemma compress_normalize_primitive_monad_None: 
+      assumes "\<And>m m' f. f \<in> set fs \<Longrightarrow> normalized_nnf_match m \<Longrightarrow> f m = Some m' \<Longrightarrow> matches \<gamma> m' a p \<longleftrightarrow> matches \<gamma> m a p"
+          and "\<And>m f. f \<in> set fs \<Longrightarrow> normalized_nnf_match m \<Longrightarrow> f m = None \<Longrightarrow> \<not> matches \<gamma> m a p"
+          and "\<And>m m' f. f \<in> set fs \<Longrightarrow> normalized_nnf_match m \<Longrightarrow> f m = Some m' \<Longrightarrow> normalized_nnf_match m'"
+          and "normalized_nnf_match m"
+          and "(compress_normalize_primitive_monad fs m) = None"
+      shows "\<not> matches \<gamma> m a p"
+    using assms proof(induction fs arbitrary: m)
+    case Nil thus ?case by simp
+    next
+    case (Cons f fs)
+      from Cons.prems(1) have IH_prem1:
+        "(\<And>f m m'. f \<in> set fs \<Longrightarrow> normalized_nnf_match m \<Longrightarrow> f m = Some m' \<Longrightarrow> matches \<gamma> m' a p = matches \<gamma> m a p)" by auto
+      from Cons.prems(2) have IH_prem2:
+        "(\<And>f m m'. f \<in> set fs \<Longrightarrow> normalized_nnf_match m \<Longrightarrow> f m = None \<Longrightarrow> \<not> matches \<gamma> m a p)" by auto
+      from Cons.prems(3) have IH_prem3:
+        "(\<And>f m m'. f \<in> set fs \<Longrightarrow> normalized_nnf_match m \<Longrightarrow> f m = Some m' \<Longrightarrow> normalized_nnf_match m')" by auto
+      from Cons.IH IH_prem1 IH_prem2 IH_prem3 have
+        IH: "\<And>m. normalized_nnf_match m \<Longrightarrow> compress_normalize_primitive_monad fs m = None \<Longrightarrow> \<not>  matches \<gamma> m a p" by blast
+      show ?case
+        proof(cases "f m")
+          case None thus ?thesis using Cons.prems(4) Cons.prems(2) Cons.prems(3) by auto
+        next
+          case(Some m'')
+            from Some Cons.prems(3)[of f] Cons.prems(4) have 2: "normalized_nnf_match m''" by simp
+            from Some have "compress_normalize_primitive_monad (f # fs) m = compress_normalize_primitive_monad fs m''" by simp
+            hence "\<not> matches \<gamma> m'' a p" using Cons.prems(5) IH 2 by simp
+            thus ?thesis using Cons.prems(1) Cons.prems(4) Some by auto 
+        qed
+    qed
+
+
+lemma compress_normalize_primitive_monad_preserves:
+      assumes "\<And>m m' f. f \<in> set fs \<Longrightarrow> normalized_nnf_match m \<Longrightarrow> f m = Some m' \<Longrightarrow> normalized_nnf_match m'"
+          and "\<And>m m' f. f \<in> set fs \<Longrightarrow> normalized_nnf_match m \<Longrightarrow> P m \<Longrightarrow> f m = Some m' \<Longrightarrow> P m'"
+          and "normalized_nnf_match m"
+          and "P m"
+          and "(compress_normalize_primitive_monad fs m) = Some m'"
+      shows "normalized_nnf_match m' \<and> P m'"
+    using assms proof(induction fs arbitrary: m)
+    case Nil thus ?case by simp
+    next
+    case (Cons f fs) thus ?case by(simp split: option.split_asm) blast (*1s*)
+    qed
+    
 
 end
